FO-proof-systems/Sema.thy
@@ -10,9 +10,10 @@ Thus, there are no unsuitable assignments.\<close>
 term "Nil"
 
 term "None"
-
-locale formula_semantics = formula_syntax subst
+                                
+locale formula_semantics = formula_syntax subst vars
   for subst::"'v \<Rightarrow> 'c \<Rightarrow> 'p \<Rightarrow> 'p"
+  and vars ::"'p \<Rightarrow> 'v set"
   +
   fixes dom::"'t \<Rightarrow> 'c list"
 begin
